
\documentclass[a4paper,12pt]{article} % добавить leqno в [] для нумерации слева

\usepackage[left=2cm,right=2cm,
top=2cm,bottom=2cm,bindingoffset=0cm]{geometry}

\usepackage{amsmath,amsfonts,amssymb,amsthm,mathtools} % AMS
\usepackage{icomma} 
\mathtoolsset{showonlyrefs=true} % Показывать номера только у тех формул, на которые есть \eqref{} в тексте.
\usepackage{euscript}	 % Шрифт Евклид
\usepackage{mathrsfs} % Красивый матшрифт
\usepackage{enumitem}
\usepackage{siunitx}
\usepackage{tikz} % To generate the plot from csv
\usepackage{pgfplots}

\usepackage{multicol}
\setlength{\columnsep}{1cm}


%%% Заголовок
\author{Kseniia Kasianova}
\title{Microeconomics. Homework 1}
\date{\today}

\newcommand{\latinword}[1]{\textsf{\itshape #1}}%

\begin{document}

{\color{blue} \latinword{Begin to write your assignment here}}

\noindent\makebox[\linewidth]{\rule{\textwidth}{0.4pt}}


\subsection*{Problem 1}

The Cobb-Douglas production function
\[ f(z_1, z_2) = z_1^{\alpha_1} z_2^{\alpha_2} \]
where for $ l = 1, 2 $, $ z_l $ is an input, and $ \alpha_l $ is a parameter such that $ \alpha_l > 0 $ .

\begin{enumerate}
	\item 	 The firm produces with decreasing returns to scale if: 
 \begin{align*}
	   f(\lambda z_1, \lambda z_2) &< \lambda f(z_1, z_2) \\
	   (\lambda z_1)^{\alpha_1} (\lambda z_2)^{\alpha_2} &< \lambda z_1^{\alpha_1} z_2^{\alpha_2} \\
	   \lambda^{\alpha_1 + \alpha_2} z_1^{\alpha_1} z_2^{\alpha_2} &< \lambda z_1^{\alpha_1} z_2^{\alpha_2} \\
	   	   \lambda^{\alpha_1 + \alpha_2}  &< \lambda \\
	   	   \alpha_1 + \alpha_2  &< 1
 \end{align*}
	 We assume  that this condition holds.
	\item To calculate the conditional factor demand (on the quantity produced
	$ q $) we need to solve following optimization problem: 
		\begin{equation}
	\begin{cases}
	\arg \min_{(z_1,z_2) \in \mathbb{R}^2_+  }{z_1 w_1 + z_2 w_2} \\ 
	s.t.: q =  z_1^{\alpha_1} z_2^{\alpha_2} 
	\end{cases} 
	\end{equation}
	where $ w_1, w_2 $ are the prices of factors. 
	 
	The  Lagrangian for this problem: 
	\[  \mathcal{L} =   z_1 w_1 + z_2 w_2 + \lambda  ( q - z_1^{\alpha_1} z_2^{\alpha_2} ) \]
	FOC: 
	\begin{align*}
	 \begin{cases}
	 \mathcal{L}'_{z_1 } & =  w_1  -  \lambda \alpha_1 z_1^{\alpha_1-1} z_2^{\alpha_2}  = 0    \\
	\mathcal{L}'_{z_2 } & =  w_2  -  \lambda z_1^{\alpha_1} \alpha_2 z_2^{\alpha_2-1}  = 0  \\
 \mathcal{L}'_{\lambda} & = q - z_1^{\alpha_1} z_2^{\alpha_2} = 0 
\end{cases}
		\end{align*}
We get: 
	\begin{align*}
	\dfrac{w_1 }{w_2} & =  \dfrac{ \alpha_1 \hat{z}_1^{\alpha_1-1} \hat{z}_2^{\alpha_2} }{\hat{z}_1^{\alpha_1} \alpha_2 \hat{z}_2^{\alpha_2-1}} = \dfrac{ \alpha_1 \hat{z}_2}{ \alpha_2 \hat{z}_1} \Rightarrow \hat{z}_2 = \dfrac{a_2 w_1}{a_1 w_2}  \hat{z}_1  \\
q & = \hat{z}_1^{\alpha_1} \hat{z}_2^{\alpha_2}  
	\end{align*}
	That is: 
	\begin{equation}
	\begin{split}
	q  &= \hat{z}_1^{\alpha_1}  \left( \dfrac{a_2 w_1}{a_1 w_2}  \hat{z}_1 \right) ^{\alpha_2}  =  \hat{z}_1^{\alpha_1 + \alpha_2}  \left( \dfrac{a_2 w_1}{a_1 w_2}  \right) ^{\alpha_2}  \\ 
	\hat{z}_1 &=  q^{\frac{1}{a_1+a_2}} \left( \dfrac{a_1 w_2}{a_2 w_1} \right) ^{\frac{a_2}{a_1+a_2}} 
	\end{split}
	\begin{split}
 		q  &= \left( \dfrac{a_1 w_2}{a_2 w_1}  \hat{z}_2 \right) ^{\alpha_1} \hat{z}_2^{\alpha_2}    =  \hat{z}_2^{\alpha_1 + \alpha_2}  \left( \dfrac{a_1 w_2}{a_2 w_1}  \right) ^{\alpha_1}  \\ 
\hat{z}_2 &=  q^{\frac{1}{a_1+a_2}} \left( \dfrac{a_2 w_1}{a_1 w_2} \right) ^{\frac{a_1}{a_1+a_2}}	
 \end{split}
	\end{equation}
	where $ \alpha_1 + \alpha_2  < 1 $
	
	\newpage
	
	The cost
	function:
\begin{multline*}
  C(w_1, w_2, q) = w_1 \hat{z}_1  +  w_2 \hat{z}_2 \\ =   
 w_1 
 q^{\frac{1}{a_1+a_2}} \left( \dfrac{a_1 w_2}{a_2 w_1} \right) ^{\frac{a_2}{a_1+a_2}}  + w_2 q^{\frac{1}{a_1+a_2}} \left( \dfrac{a_2 w_1}{a_1 w_2} \right) ^{\frac{a_1}{a_1+a_2}} \\
 	=  w_1^{\frac{a_1}{a_1+a_2}} w_2^{\frac{a_2}{a_1+a_2}} 
 q^{\frac{1}{a_1+a_2}} \left( \dfrac{a_1 }{a_2 } \right) ^{\frac{a_2}{a_1+a_2}}  + w_1^{\frac{a_1}{a_1+a_2}} w_2^{\frac{a_2}{a_1+a_2}} q^{\frac{1}{a_1+a_2}} \left( \dfrac{a_2 }{a_1 } \right) ^{\frac{a_1}{a_1+a_2}}	\\
 = 	 w_1^{\frac{a_1}{a_1+a_2}} w_2^{\frac{a_2}{a_1+a_2}} 
 q^{\frac{1}{a_1+a_2}} \left( \left( \dfrac{a_1 }{a_2 } \right) ^{\frac{a_2}{a_1+a_2}}  +  \left( \dfrac{a_2 }{a_1 } \right) ^{\frac{a_1}{a_1+a_2}} \right) 
\end{multline*} 
where $ \alpha_1 + \alpha_2  < 1 $

	
	
	
	 Profit function: 
	 \[ \Pi(q) = pq - C(w_1, w_2, q)   = pq -  w_1^{\frac{a_1}{a_1+a_2}} w_2^{\frac{a_2}{a_1+a_2}} 
	 q^{\frac{1}{a_1+a_2}} \left( \left( \dfrac{a_1 }{a_2 } \right) ^{\frac{a_2}{a_1+a_2}}  +  \left( \dfrac{a_2 }{a_1 } \right) ^{\frac{a_1}{a_1+a_2}} \right) \]
	 where $ \alpha_1 + \alpha_2  < 1 $
	 
	 
	 Supply function: 
 \begin{align*}
  p(q) &= MC(q) = C'_q = w_1^{\frac{a_1}{a_1+a_2}} w_2^{\frac{a_2}{a_1+a_2}} 
  \dfrac{1}{a_1+a_2} q^{\frac{1-a_1-a_2}{a_1+a_2}} \left( \left( \dfrac{a_1 }{a_2 } \right) ^{\frac{a_2}{a_1+a_2}}  +  \left( \dfrac{a_2 }{a_1 } \right) ^{\frac{a_1}{a_1+a_2}} \right)  
 \end{align*}
where $ \alpha_1 + \alpha_2  < 1 $
\end{enumerate}

\subsection*{Problem 2}

The production function
\[ f(z_1,z_2) = (z_1^\rho + z_2^\rho)^{\frac{1}{\rho}} \]
where $ \rho \leqslant 1 $

\begin{enumerate}
	\item The producer profit maximization problem: 
				\begin{equation}
	\max{\Pi(q) = pq - C(w_1, w_2, q)} 
	\end{equation}
	where $ w_1, w_2 $ are prices of inputs respectively.
	\item 	To compute the demand for inputs we need to solve following optimization problem: 
	\begin{equation}
	\begin{cases}
	\arg \min_{(z_1,z_2) \in \mathbb{R}^2_+  }{z_1 w_1 + z_2 w_2} \\ 
	s.t.: q =  (z_1^\rho + z_2^\rho)^{\frac{1}{\rho}}
	\end{cases} 
	\end{equation}
	The  Lagrangian for this problem: 
	\[  \mathcal{L} =   z_1 w_1 + z_2 w_2 + \lambda  ( q - (z_1^\rho +  z_2^\rho)^{\frac{1}{\rho}} ) \]
	FOC: 
	\begin{align*}
	\begin{cases}
	\mathcal{L}'_{z_1 } & =  w_1  -  \lambda z_1^{\rho-1} (z_1^\rho+z_2^\rho)^{\frac{1}{\rho} - 1 }  = 0    \\
	\mathcal{L}'_{z_2 } & =  w_2  -  \lambda z_2^{\rho-1} (z_1^\rho+z_2^\rho)^{\frac{1}{\rho} - 1 }  = 0  \\
	\mathcal{L}'_{\lambda} & = q - (z_1^\rho + z_2^\rho)^{\frac{1}{\rho}} = 0 
	\end{cases}
	\end{align*}
	We get: 
	\begin{align*}
	\dfrac{w_1 }{w_2} & =  \dfrac{ \hat{z}_1^{\rho-1} (\hat{z}_1^\rho+\hat{z}_2^\rho)^{\frac{1}{\rho} - 1 } }{\hat{z}_2^{\rho-1} (\hat{z}_1^\rho+\hat{z}_2^\rho)^{\frac{1}{\rho} - 1 } } = \dfrac{ \hat{z}_1^{\rho-1}  }{\hat{z}_2^{\rho-1}  } \Rightarrow \hat{z}_2 = \left( \dfrac{w_2} { w_1} \right) ^{\frac{1}{\rho}-1} \hat{z}_1  \\
	q & = (\hat{z}_1^\rho + \hat{z}_2^\rho)^{\frac{1}{\rho}}   
	\end{align*}
	That is: 
	\begin{align*}
	q  &= \hat{z}_1^{\rho}  \left( 1 + \left( \dfrac{w_2}{w_1}   \right) ^{\frac{\rho}{\alpha}} \right) \\ 
	\hat{z}_1 &=  q^{\frac{1}{\rho}}  \left( 1 + \left( \dfrac{w_2}{w_1}   \right) ^{\frac{\rho}{\alpha}} \right)^{-\frac{1}{\rho}} \\   
	\hat{z}_2 &=  q^{\frac{1}{\rho}}  \left( 1 + \left( \dfrac{w_1}{w_2}   \right) ^{\frac{\rho}{\alpha}} \right)^{-\frac{1}{\rho}}
			\end{align*}
	\item The cost
	function:
	\begin{multline*}
	C(w_1, w_2, q) = w_1 \hat{z}_1  +  w_2 \hat{z}_2 =   
	w_1 
	q^{\frac{1}{\rho}}  \left( 1 +  \left( \dfrac{w_2}{w_1}   \right) ^{\frac{\rho}{\alpha}} \right)^{-\frac{1}{\rho}}  + w_2 q^{\frac{1}{\rho}}  \left( 1 + \left( \dfrac{w_1}{w_2}   \right) ^{\frac{\rho}{\alpha}} \right)^{-\frac{1}{\rho}}  
	\end{multline*} 
	\end{enumerate}



\end{document}